src/proof/k8s_io/apimachinery/pkg/apis/meta/v1.v
@@ -570,6 +570,380 @@ Lemma wp_DeleteOptions__DeepCopy l options :
   }}}.
 Proof. Admitted.
 
+Lemma wp_GetOwnerReferences_deepown l m dq :
+  {{{ is_pkg_init v1 ∗
+      ObjectMetaV.deepown_l l m dq
+  }}}
+    l @! (go.PointerType v1.ObjectMeta) @! "GetOwnerReferences" #()
+  {{{ sl, RET #sl;
+      ⌜ sl = slice.nil ↔ m.(ObjectMetaV.OwnerReferences') = None ⌝ ∗
+      match m.(ObjectMetaV.OwnerReferences') with
+      | Some refs => ∃ cs,
+          sl ↦*{dq} cs ∗
+          ([∗ list] c;ref ∈ cs;refs, OwnerReferenceV.deepown c ref dq) ∗
+          (∀ cs', sl ↦*{dq} cs' ∗
+           ([∗ list] c;ref ∈ cs';refs, OwnerReferenceV.deepown c ref dq) -∗
+           ObjectMetaV.deepown_l l m dq)
+      | None => ObjectMetaV.deepown_l l m dq
+      end
+  }}}.
+Proof.
+  iIntros (Φ) "(#Hinit & Hmeta) HΦ".
+  iDestruct "Hmeta" as (c) "[Hl Hmeta]".
+  wp_method_call. rewrite /v1.ObjectMeta__GetOwnerReferencesⁱᵐᵖˡ. wp_call.
+  iNamed "Hmeta". wp_auto.
+  iApply "HΦ". iSplit; first done.
+  destruct m.(ObjectMetaV.OwnerReferences') as [refs|] eqn:Hrefs.
+  - iDestruct "Hdeepown_ownerreferences_some" as (cs) "[Hsl Hrefs]".
+    iExists cs. iFrame. iIntros (cs') "[Hsl Hrefs]".
+    iExists c. iFrame. iFrame "%". iSplit.
+    + iPureIntro. rewrite Hrefs. exact Hdeepown_ownerreferences_none.
+    + rewrite Hrefs. iExists cs'. iFrame.
+  - iExists c. iFrame. iFrame "%". iSplit.
+    + iPureIntro. rewrite Hrefs. exact Hdeepown_ownerreferences_none.
+    + rewrite Hrefs. iFrame.
+Qed.
+
+Definition is_controller_reference_of (m : ObjectMetaV.t)
+    (ref : OwnerReferenceV.t) : Prop :=
+  ∃ refs,
+    m.(ObjectMetaV.OwnerReferences') = Some refs ∧
+    ref ∈ refs ∧
+    ref.(OwnerReferenceV.Controller') = Some true.
+
+Definition owner_references_borrow (m : ObjectMetaV.t) (dq : dfrac)
+    (sl : slice.t)
+    (Restore : iProp Σ) : iProp Σ :=
+  ⌜ sl = slice.nil ↔ m.(ObjectMetaV.OwnerReferences') = None ⌝ ∗
+  match m.(ObjectMetaV.OwnerReferences') with
+  | Some refs => ∃ cs,
+      sl ↦*{dq} cs ∗
+      ([∗ list] c;ref ∈ cs;refs, OwnerReferenceV.deepown c ref dq) ∗
+      (∀ cs',
+        sl ↦*{dq} cs' ∗
+        ([∗ list] c;ref ∈ cs';refs, OwnerReferenceV.deepown c ref dq) -∗
+        Restore)
+  | None => Restore
+  end.
+
+Definition get_owner_references_capability (owner : interface.t)
+    (m : ObjectMetaV.t) (dq : dfrac)
+    (Own : iProp Σ) : iProp Σ :=
+  {{{ "Hinit" ∷ is_pkg_init v1 ∗
+      "Hown" ∷ Own
+  }}}
+    (MethodResolve v1.Object "GetOwnerReferences" #owner) #()
+  {{{ sl, RET #sl; owner_references_borrow m dq sl Own }}}.
+
+Lemma get_owner_references_capability_ObjectMeta meta_l m dq :
+  ⊢ get_owner_references_capability
+    (interface.mk_ok (go.PointerType v1.ObjectMeta) #meta_l) m dq
+    (ObjectMetaV.deepown_l meta_l m dq).
+Proof.
+  unfold get_owner_references_capability.
+  wp_start as "H".
+  iNamed "H".
+  wp_auto.
+  wp_apply (wp_GetOwnerReferences_deepown with "[$Hinit $Hown]").
+  iIntros (sl) "Hrefs".
+  iApply "HΦ". iExact "Hrefs".
+Qed.
+
+Local Lemma wp_GetControllerOfNoCopy_general owner m dq (Own : iProp Σ) :
+  {{{ "Hinit" ∷ is_pkg_init v1 ∗
+      "Hget" ∷ get_owner_references_capability owner m dq Own ∗
+      "Hmeta" ∷ Own
+  }}}
+    @! v1.GetControllerOfNoCopy #owner
+  {{{ controller_ref_l, RET #controller_ref_l;
+      (⌜ controller_ref_l = null ⌝ ∗
+       Own) ∨
+      (∃ controller_ref controller_c,
+        ⌜ controller_ref_l ≠ null ∧ is_controller_reference_of m controller_ref ⌝ ∗
+        controller_ref_l ↦{dq} controller_c ∗
+        OwnerReferenceV.deepown controller_c controller_ref dq ∗
+        (controller_ref_l ↦{dq} controller_c ∗
+         OwnerReferenceV.deepown controller_c controller_ref dq -∗ Own))
+  }}}.
+Proof.
+  wp_start as "H". iNamed "H".
+  rewrite exception_do_unseal /exception_do_def.
+  wp_alloc controllee_ptr as "Hcontrollee".
+  wp_pures.
+  wp_alloc refs_ptr as "Hrefs_ptr".
+  wp_pures.
+  wp_load.
+  wp_apply ("Hget" with "[$Hinit $Hmeta]").
+  iIntros (refs_sl) "(%Hrefs_nil & Hrefs)". wp_auto.
+  destruct m.(ObjectMetaV.OwnerReferences') as [refs|] eqn:Hrefs_some.
+  2: {
+    assert (refs_sl = slice.nil) as ->.
+    { apply Hrefs_nil. done. }
+    iPoseProof (own_slice_nil (V:=v1.OwnerReference.t) dq) as "Hrefs_sl".
+    wp_alloc loop_i_ptr as "Hloop_i". wp_auto.
+    set I0 := (∃ (loop_i : w64),
+      "Hloop_i" ∷ loop_i_ptr ↦ loop_i ∗
+      "%Hloop_i_bound" ∷ ⌜ 0 ≤ sint.Z loop_i ⌝)%I.
+    iAssert I0 with "[Hloop_i]" as "Hloop".
+    { iExists (W64 0). iFrame. iPureIntro. word. }
+    wp_for "Hloop". wp_if_destruct; first word.
+    clear I0. wp_auto.
+    rewrite return_val_unseal /return_val_def. wp_auto.
+    iApply "HΦ". iLeft. iFrame. done. }
+  iDestruct "Hrefs" as (cs) "(Hrefs_sl & Hrefs & Hmeta_restore)".
+  iDestruct (own_slice_len with "Hrefs_sl") as %(Hrefs_len1 & Hrefs_len2).
+  iDestruct (big_sepL2_length with "Hrefs") as %Hrefs_len.
+  wp_alloc loop_i_ptr as "Hloop_i". wp_auto.
+  set I := (∃ (loop_i source_i : w64),
+    "Hloop_i" ∷ loop_i_ptr ↦ loop_i ∗
+    "Hi" ∷ i_ptr ↦ source_i ∗
+    "Hrefs_sl" ∷ refs_sl ↦*{dq} cs ∗
+    "Hrefs" ∷ ([∗ list] c;ref ∈ cs;refs, OwnerReferenceV.deepown c ref dq) ∗
+    "%Hi_bound" ∷ ⌜ 0 ≤ sint.Z loop_i ≤ sint.Z (slice.len refs_sl) ⌝)%I.
+  iAssert I with "[Hloop_i i Hrefs_sl Hrefs]" as "Hloop".
+  { iExists (W64 0), (W64 0). iFrame. iPureIntro. word. }
+  wp_for "Hloop". wp_if_destruct.
+  - list_elem cs (sint.Z loop_i) as this_c.
+    destruct (decide (0 ≤ sint.Z loop_i < sint.Z (slice.len refs_sl)))
+      as [_|Hbounds]; last word.
+    wp_apply (wp_load_slice_index with "[$Hrefs_sl]"); [word| |].
+    { iPureIntro. exact Hthis_c_lookup. }
+    iIntros "Hrefs_sl". wp_auto.
+    assert (∃ this_ref, refs !! sint.nat loop_i = Some this_ref) as
+      [this_ref Hthis_ref_lookup].
+    { apply lookup_lt_is_Some_2. rewrite -Hrefs_len Hrefs_len1. word. }
+    iDestruct (big_sepL2_lookup_acc with "Hrefs") as "[Hthis Hrefs_close]";
+      [exact Hthis_c_lookup|exact Hthis_ref_lookup|].
+    iDestruct (own_slice_elem_acc (sint.Z loop_i) with "Hrefs_sl")
+      as "[Hcell Hrefs_sl_close]"; [word|exact Hthis_c_lookup|].
+    iDestruct (typed_pointsto_not_null with "Hcell") as %Hthis_c_nonnull.
+    iNamedPrefix "Hthis" "Hthis_".
+    destruct this_ref.(OwnerReferenceV.Controller') as [controller|]
+      eqn:Hcontroller.
+    + iDestruct "Hthis_Hdeepown_controller_some" as
+        (controller_c) "[Hcontroller %Hcontroller_c]".
+      subst controller_c.
+      assert (this_c.(v1.OwnerReference.Controller') ≠ null) as Hcontroller_nonnull.
+      { intros Hnull. apply Hthis_Hdeepown_controller_none in Hnull.
+        done. }
+      destruct controller.
+      * destruct (decide
+          (0 ≤ sint.Z loop_i < sint.Z (slice.len refs_sl)))
+        as [_|Hbounds']; last word.
+        wp_auto.
+        rewrite -> bool_decide_false by exact Hcontroller_nonnull.
+        wp_auto.
+        destruct (decide
+          (0 ≤ sint.Z loop_i < sint.Z (slice.len refs_sl)))
+          as [_|Hbounds'']; last word.
+        wp_auto.
+        iCombineNamed "Hthis_*" as "Hthis".
+        destruct (decide
+          (0 ≤ sint.Z loop_i < sint.Z (slice.len refs_sl)))
+          as [_|Hbounds''']; last word.
+        wp_auto.
+        iApply wp_for_post_return.
+        rewrite return_val_unseal /return_val_def. wp_auto.
+        rewrite exception_seq_unseal /exception.exception_seq_def. wp_auto.
+        iApply ("HΦ" $! (slice_index_ref v1.OwnerReference.t
+          (sint.Z loop_i) refs_sl)). iRight.
+        iExists this_ref, this_c. iSplitR.
+        { iPureIntro. split; first exact Hthis_c_nonnull.
+          unfold is_controller_reference_of. eexists. split; first done.
+          split; [eapply list_elem_of_lookup_2; exact Hthis_ref_lookup|done]. }
+        iFrame "Hcell".
+        iAssert (OwnerReferenceV.deepown this_c this_ref dq)
+          with "[Hthis Hcontroller]" as "Hthis".
+        { unfold OwnerReferenceV.deepown. iFrame "% Hthis".
+          iSplit.
+          - iPureIntro. rewrite Hcontroller.
+            exact Hthis_Hdeepown_controller_none.
+          - rewrite Hcontroller. iExists true. iFrame. done. }
+        iFrame "Hthis".
+        iIntros "[Hcell Hthis]".
+        iDestruct ("Hrefs_sl_close" with "Hcell") as "Hrefs_sl".
+        iDestruct ("Hrefs_close" with "Hthis") as "Hrefs".
+        iEval (rewrite (list_insert_id _ _ _ Hthis_c_lookup)) in "Hrefs_sl".
+        iApply ("Hmeta_restore" $! cs). iFrame.
+      * destruct (decide
+          (0 ≤ sint.Z loop_i < sint.Z (slice.len refs_sl)))
+        as [_|Hbounds']; last word.
+        wp_auto.
+        rewrite -> bool_decide_false by exact Hcontroller_nonnull.
+        wp_auto.
+        destruct (decide
+          (0 ≤ sint.Z loop_i < sint.Z (slice.len refs_sl)))
+          as [_|Hbounds'']; last word.
+        wp_auto.
+        iCombineNamed "Hthis_*" as "Hthis_rest".
+        iAssert (OwnerReferenceV.deepown this_c this_ref dq)
+          with "[Hthis_rest Hcontroller]" as "Hthis".
+        { unfold OwnerReferenceV.deepown. iFrame "% Hthis_rest".
+          iSplit.
+          - iPureIntro. rewrite Hcontroller.
+            exact Hthis_Hdeepown_controller_none.
+          - rewrite Hcontroller. iExists false. iFrame. done. }
+        iDestruct ("Hrefs_sl_close" with "Hcell") as "Hrefs_sl".
+        iDestruct ("Hrefs_close" with "Hthis") as "Hrefs".
+        iEval (rewrite (list_insert_id _ _ _ Hthis_c_lookup)) in "Hrefs_sl".
+        iApply wp_for_post_do. wp_auto.
+        iFrame "HΦ Hmeta_restore Hrefs_ptr".
+        iExists (word.add loop_i (W64 1)), loop_i. iFrame. iPureIntro. word.
+    + assert (this_c.(v1.OwnerReference.Controller') = null) as Hcontroller_null.
+      { apply Hthis_Hdeepown_controller_none. done. }
+      destruct (decide
+        (0 ≤ sint.Z loop_i < sint.Z (slice.len refs_sl)))
+        as [_|Hbounds']; last word.
+      wp_auto.
+      rewrite -> bool_decide_true by exact Hcontroller_null.
+      wp_auto.
+      iAssert (OwnerReferenceV.deepown this_c this_ref dq)
+        with "[Hthis_Hdeepown_blockownerdeleton_some]" as "Hthis".
+      { unfold OwnerReferenceV.deepown.
+        iFrame "% Hthis_Hdeepown_blockownerdeleton_some".
+        iSplit.
+        - iPureIntro. rewrite Hcontroller.
+          exact Hthis_Hdeepown_controller_none.
+        - rewrite Hcontroller. done. }
+      iDestruct ("Hrefs_sl_close" with "Hcell") as "Hrefs_sl".
+      iDestruct ("Hrefs_close" with "Hthis") as "Hrefs".
+      iEval (rewrite (list_insert_id _ _ _ Hthis_c_lookup)) in "Hrefs_sl".
+      iApply wp_for_post_do. wp_auto.
+      iFrame "HΦ Hmeta_restore Hrefs_ptr".
+      iExists (word.add loop_i (W64 1)), loop_i. iFrame. iPureIntro. word.
+  - clear I.
+    rewrite return_val_unseal /return_val_def. wp_auto.
+    iApply "HΦ". iLeft. iSplit; first done.
+    iApply ("Hmeta_restore" $! cs). iFrame.
+Qed.
+
+Lemma wp_GetControllerOf_general owner m dq (Own : iProp Σ) :
+  {{{ "Hinit" ∷ is_pkg_init v1 ∗
+      "Hget" ∷ get_owner_references_capability owner m dq Own ∗
+      "Hmeta" ∷ Own
+  }}}
+    @! v1.GetControllerOf #owner
+  {{{ controller_ref_l, RET #controller_ref_l;
+      Own ∗
+      (⌜ controller_ref_l = null ⌝ ∨
+       ∃ controller_ref,
+         ⌜ controller_ref_l ≠ null ∧ is_controller_reference_of m controller_ref ⌝ ∗
+         OwnerReferenceV.deepown_l controller_ref_l controller_ref 1)
+  }}}.
+Proof.
+  wp_start as "H". iNamed "H".
+  wp_auto.
+  wp_bind (@! v1.GetControllerOfNoCopy #owner)%E.
+  wp_apply (wp_GetControllerOfNoCopy_general owner m dq Own with
+    "[$Hinit $Hget $Hmeta]").
+  iIntros (controller_ref_l) "Hresult".
+  iDestruct "Hresult" as "[(%Hnull & Hmeta)|Hresult]".
+  - subst controller_ref_l. wp_auto. iApply "HΦ". iFrame "Hmeta".
+    iLeft. done.
+  - iDestruct "Hresult" as (controller_ref controller_c)
+      "(%Hcontroller & Href_l & Href & Hrestore)".
+    destruct Hcontroller as [Hcontroller_l_nonnull Hcontroller].
+    wp_auto.
+    rewrite -> bool_decide_false by exact Hcontroller_l_nonnull.
+    wp_auto.
+    unfold is_controller_reference_of in Hcontroller.
+    destruct Hcontroller as (refs & Hrefs_some & Hcontroller_mem & Hcontroller).
+    iNamedPrefix "Href" "Href_".
+    iEval (rewrite Hcontroller) in "Href_Hdeepown_controller_some".
+    iDestruct "Href_Hdeepown_controller_some" as
+      (controller_b) "[Hcontroller_b %Hcontroller_b]".
+    subst controller_b.
+    wp_auto.
+    wp_bind (#(functions ptr.To [go.bool]) #true)%E.
+    wp_func_call. wp_call. wp_auto.
+    destruct controller_ref.(OwnerReferenceV.BlockOwnerDeletion') as [block|]
+      eqn:Hblock.
+    + iDestruct "Href_Hdeepown_blockownerdeleton_some" as
+        (block_c) "[Hblock_c %Hblock_c]". subst block_c.
+      iDestruct (typed_pointsto_not_null with "Hblock_c") as %Hblock_nonnull.
+      rewrite -> bool_decide_false by exact Hblock_nonnull.
+      wp_auto.
+      wp_bind (#(functions ptr.To [go.bool]) #block)%E.
+      wp_func_call. wp_call.
+      wp_alloc block_ptr as "Hblock_new". wp_auto.
+      iAssert (OwnerReferenceV.deepown controller_c controller_ref dq)
+        with "[Hcontroller_b Hblock_c]" as "Href".
+      { unfold OwnerReferenceV.deepown, named. iFrame "%".
+        rewrite Hcontroller. iSplitL "Hcontroller_b".
+        - iExists true. iFrame. done.
+        - iSplitL "".
+          + iPureIntro. rewrite Hblock.
+            exact Href_Hdeepown_blockownerdeleton_none.
+          + rewrite Hblock. iExists block. iFrame. done. }
+      iDestruct ("Hrestore" with "[$Href_l $Href]") as "Hmeta".
+      iDestruct (typed_pointsto_not_null with "v") as %Hv_nonnull.
+      iDestruct (typed_pointsto_not_null with "Hblock_new") as %Hblock_new_nonnull.
+      iDestruct (typed_pointsto_not_null with "cp") as %Hcp_nonnull.
+      iApply "HΦ". iFrame "Hmeta". iRight.
+      iExists controller_ref. iSplitR.
+      { iPureIntro. split; first exact Hcp_nonnull. unfold is_controller_reference_of.
+        eexists. done. }
+      iExists (controller_c <| v1.OwnerReference.Controller' := v_ptr |> <|
+        v1.OwnerReference.BlockOwnerDeletion' := block_ptr |>).
+      iFrame "cp". unfold OwnerReferenceV.deepown, named. simpl.
+      iFrame "%". rewrite Hcontroller Hblock.
+      iSplitL "".
+      * iPureIntro. split; intros; done.
+      * iSplitL "v".
+        { iExists true. iFrame. done. }
+        iSplitL "".
+        { iPureIntro. split; intros; done. }
+        iExists block. iFrame. done.
+    + assert (controller_c.(v1.OwnerReference.BlockOwnerDeletion') = null)
+        as Hblock_null.
+      { apply Href_Hdeepown_blockownerdeleton_none. done. }
+      rewrite -> bool_decide_true by exact Hblock_null.
+      wp_auto.
+      iAssert (OwnerReferenceV.deepown controller_c controller_ref dq)
+        with "[Hcontroller_b]" as "Href".
+      { unfold OwnerReferenceV.deepown, named. iFrame "%".
+        rewrite Hcontroller Hblock. iSplitL "Hcontroller_b".
+        - iExists true. iFrame. done.
+        - iSplitL "".
+          + iPureIntro. exact Href_Hdeepown_blockownerdeleton_none.
+          + done. }
+      iDestruct ("Hrestore" with "[$Href_l $Href]") as "Hmeta".
+      iDestruct (typed_pointsto_not_null with "v") as %Hv_nonnull.
+      iDestruct (typed_pointsto_not_null with "cp") as %Hcp_nonnull.
+      iApply "HΦ". iFrame "Hmeta". iRight.
+      iExists controller_ref. iSplitR.
+      { iPureIntro. split; first exact Hcp_nonnull. unfold is_controller_reference_of.
+        eexists. done. }
+      iExists (controller_c <| v1.OwnerReference.Controller' := v_ptr |>).
+      iFrame "cp". unfold OwnerReferenceV.deepown, named. simpl.
+      iFrame "%". rewrite Hcontroller Hblock.
+      iSplitL "".
+      * iPureIntro. split; intros; done.
+      * iSplitL "v".
+        { iExists true. iFrame. done. }
+        iSplitL ""; done.
+Qed.
+
+Lemma wp_GetControllerOf owner meta_l m dq :
+  {{{ "Hinit" ∷ is_pkg_init v1 ∗
+      "%Howner" ∷ ⌜ owner = interface.mk_ok (go.PointerType v1.ObjectMeta) #meta_l ⌝ ∗
+      "Hmeta" ∷ ObjectMetaV.deepown_l meta_l m dq
+  }}}
+    @! v1.GetControllerOf #owner
+  {{{ controller_ref_l, RET #controller_ref_l;
+      ObjectMetaV.deepown_l meta_l m dq ∗
+      (⌜ controller_ref_l = null ⌝ ∨
+       ∃ controller_ref,
+         ⌜ controller_ref_l ≠ null ∧ is_controller_reference_of m controller_ref ⌝ ∗
+         OwnerReferenceV.deepown_l controller_ref_l controller_ref 1)
+  }}}.
+Proof.
+  iIntros (Φ) "H HΦ". iNamed "H". subst owner.
+  iPoseProof (get_owner_references_capability_ObjectMeta meta_l m dq) as "Hget".
+  iApply (wp_GetControllerOf_general with "[$Hinit $Hget $Hmeta]").
+  iExact "HΦ".
+Qed.
+
 Lemma wp_NewControllerRef_ReplicaSet owner gvk rs_l m dq:
   {{{ is_pkg_init v1 ∗
       ⌜ owner = interface.mk_ok (go.PointerType v1.ReplicaSet) (# rs_l) ⌝ ∗
@@ -581,6 +955,7 @@ Lemma wp_NewControllerRef_ReplicaSet owner gvk rs_l m dq:
       ⌜ OwnerReferenceV.refers_to_controller controller_ref gvk.(schema.GroupVersionKind.Kind')
         m.(ObjectMetaV.Name')
         m.(ObjectMetaV.UID') ⌝ ∗
+      ⌜ OwnerReferenceV.valid controller_ref ⌝ ∗
       ObjectMetaV.deepown_l (ReplicaSetV.objectmeta_ptr rs_l) m dq
   }}}.
 Proof. Admitted.
