src/proof/controllers/replicaset/get_indirectly_related_pods.v
@@ -1,0 +1,50 @@
+From New.proof Require Import prelude empty_ffi.
+From New.proof.controllers.replicaset Require Export get_replica_sets_with_same_controller.
+From New.proof.kubernetes_model Require Export inv.
+
+Section proof.
+Context `{hG: !heapGS Σ} `{!ffi_semantics _ _}.
+Context {sem : go.Semantics}
+  {package_sem : code.controllers.replicaset.replicaset.Assumptions}.
+Collection W := sem + package_sem.
+#[local] Instance base_common_sem : common.Assumptions | 100 :=
+  code.controllers.replicaset.replicaset.import_common_Assumption.
+#[local] Instance controller_sem : controller.Assumptions :=
+  code.controllers.replicaset.replicaset.import_controller_Assumption.
+#[local] Instance base_apimodel_sem : apimodel.Assumptions | 100 :=
+  common.import_apimodel_Assumption.
+#[local] Instance object_meta_v1_sem :
+    code.k8s_io.apimachinery.pkg.apis.meta.v1.v1.Assumptions :=
+  apimodel.import_apis_meta_v1_Assumption.
+#[local] Instance object_apps_v1_sem :
+    code.k8s_io.api.apps.v1.v1.Assumptions :=
+  apimodel.import_api_apps_v1_Assumption.
+#[local] Instance object_core_v1_sem :
+    code.k8s_io.api.core.v1.v1.Assumptions :=
+  code.k8s_io.api.apps.v1.v1.import_core_v1_Assumption.
+#[local] Instance apimodel_sem : apimodel.Assumptions | 0.
+Proof using package_sem.
+  constructor; try exact object_core_v1_sem; try apply _.
+Defined.
+#[local] Instance common_sem : common.Assumptions | 0.
+Proof using package_sem.
+  constructor; try exact apimodel_sem; try apply _.
+Defined.
+Context `{!kubernetesModelG Σ}.
+Local Set Default Proof Using "All".
+
+Lemma wp_getIndirectlyRelatedPods γ l rs_l rs dq :
+  {{{ is_pkg_init code.controllers.replicaset.pkg_id.replicaset ∗
+      "Hisk" ∷ is_kubernetes γ l ∗
+      "Hglobal_l" ∷ (global_addr apimodel.ModelState) ↦□ l ∗
+      "Hrs" ∷ ReplicaSetV.deepown_l rs_l rs dq
+  }}}
+    @! replicaset.getIndirectlyRelatedPods #rs_l
+  {{{ sl ptrs pods dq', RET (#sl, #interface.nil);
+      sl ↦* ptrs ∗
+      ([∗ list] ptr;pod ∈ ptrs;pods, PodV.deepown_l ptr pod dq') ∗
+      ReplicaSetV.deepown_l rs_l rs dq
+  }}}.
+Proof. Admitted.
+
+End proof.
