src/proof/controllers/replicaset/get_replica_sets_with_same_controller.v
@@ -1,0 +1,251 @@
+From New.proof Require Import prelude empty_ffi.
+From New.proof.controllers.replicaset Require Export replicaset_init.
+From New.proof.k8s_io.api.apps Require Export v1.
+From New.proof.kubernetes_types Require Export prelude.
+From New.proof.kubernetes_model Require Export list_weak.
+
+Section proof.
+Context `{hG: !heapGS Σ} `{!ffi_semantics _ _}.
+Context {sem : go.Semantics}
+  {package_sem : code.controllers.replicaset.replicaset.Assumptions}.
+Collection W := sem + package_sem.
+#[local] Instance base_common_sem : common.Assumptions | 100 :=
+  code.controllers.replicaset.replicaset.import_common_Assumption.
+#[local] Instance controller_sem : controller.Assumptions :=
+  code.controllers.replicaset.replicaset.import_controller_Assumption.
+#[local] Instance base_apimodel_sem : apimodel.Assumptions | 100 :=
+  common.import_apimodel_Assumption.
+#[local] Instance object_meta_v1_sem :
+    code.k8s_io.apimachinery.pkg.apis.meta.v1.v1.Assumptions :=
+  apimodel.import_apis_meta_v1_Assumption.
+#[local] Instance object_apps_v1_sem :
+    code.k8s_io.api.apps.v1.v1.Assumptions :=
+  apimodel.import_api_apps_v1_Assumption.
+#[local] Instance object_core_v1_sem :
+    code.k8s_io.api.core.v1.v1.Assumptions :=
+  code.k8s_io.api.apps.v1.v1.import_core_v1_Assumption.
+#[local] Instance apimodel_sem : apimodel.Assumptions | 0.
+Proof using package_sem.
+  constructor; try exact object_core_v1_sem; try apply _.
+Defined.
+#[local] Instance common_sem : common.Assumptions | 0.
+Proof using package_sem.
+  constructor; try exact apimodel_sem; try apply _.
+Defined.
+Context `{!kubernetesModelG Σ}.
+Local Set Default Proof Using "All".
+
+Lemma wp_getReplicaSetsWithSameController γ model_l rs_l rs dq :
+  {{{ is_pkg_init code.controllers.replicaset.pkg_id.replicaset ∗
+      "#Hisk" ∷ is_kubernetes γ model_l ∗
+      "#Hglobal_l" ∷ (global_addr apimodel.ModelState) ↦□ model_l ∗
+      "Hrs" ∷ ReplicaSetV.deepown_l rs_l rs dq
+  }}}
+    @! replicaset.getReplicaSetsWithSameController #rs_l
+  {{{ sl ptrs replica_sets dq', RET (#sl, #interface.nil);
+      sl ↦* ptrs ∗
+      ([∗ list] ptr;replica_set ∈ ptrs;replica_sets, ReplicaSetV.deepown_l ptr replica_set dq') ∗
+      ReplicaSetV.deepown_l rs_l rs dq
+  }}}.
+Proof.
+  wp_start as "H". iNamed "H".
+  iAssert (is_pkg_init v1) as "#Hmeta_init".
+  { iPkgInit. }
+  iAssert (is_pkg_init labels) as "#Hlabels_init".
+  { iPkgInit. }
+  iAssert (is_pkg_init apimodel) as "#Hapimodel_init".
+  { iPkgInit. }
+  wp_auto.
+  wp_bind (@! v1.GetControllerOf
+    #(interface.mk_ok (go.PointerType api_apps_v1.ReplicaSet) #rs_l))%E.
+  wp_apply (wp_GetControllerOf_ReplicaSet with
+    "[$Hmeta_init $Hrs //]").
+  iIntros (controller_ref_l) "(Hrs & Hcontroller_ref)".
+  iDestruct "Hcontroller_ref" as
+    "[%Hcontroller_ref_null|Hcontroller_ref]".
+  - subst controller_ref_l. wp_auto.
+    iApply ("HΦ" $! slice.nil [] [] (DfracOwn 1)).
+    iPoseProof (own_slice_nil (V:=loc) (DfracOwn 1)) as "Hnil".
+    simpl. iFrame. iExact "Hnil".
+  - iDestruct "Hcontroller_ref" as (controller_ref)
+      "(%Hcontroller_ref & Hcontroller_ref)".
+    destruct Hcontroller_ref as
+      [Hcontroller_ref_nonnull Hcontroller_ref_of].
+    wp_auto.
+    rewrite -> bool_decide_false by exact Hcontroller_ref_nonnull.
+    wp_auto.
+    iDestruct "Hcontroller_ref" as (controller_ref_c)
+      "[Hcontroller_ref_l Hcontroller_ref]".
+    iDestruct (struct_fields_split (V:=v1.OwnerReference.t) with
+      "Hcontroller_ref_l") as
+      "[Hcontroller_ref_fields %Hcontroller_ref_l_nonnull]".
+    iNamedPrefix "Hcontroller_ref_fields" "Hcontroller_ref_field_".
+    iNamedPrefix "Hcontroller_ref" "Hcontroller_ref_deepown_".
+    iRename "controllerRef" into "Hcontroller_var".
+    iRename "Hcontroller_ref_field_UID" into "Hcontroller_uid".
+    iCombineNamed "Hcontroller_ref_*" as "Hcontroller_rest".
+    iPoseProof (ReplicaSetV.deepown_l_split with "Hrs") as
+      "(%Hrs_l_nonnull & Hrs_typemeta & Hrs_meta_l & Hrs_spec & Hrs_status)".
+    iDestruct "Hrs_meta_l" as (rs_meta_c) "[Hrs_meta_l Hrs_meta]".
+    iDestruct (struct_fields_split (V:=v1.ObjectMeta.t) with
+      "Hrs_meta_l") as "[Hrs_meta_fields %Hrs_meta_l_nonnull]".
+    iNamedPrefix "Hrs_meta_fields" "Hrs_meta_field_".
+    iNamedPrefix "Hrs_meta" "Hrs_meta_deepown_".
+    wp_auto.
+    rewrite Hrs_meta_deepown_Hdeepown_namespace.
+    wp_bind (@! labels.Everything #())%E.
+    wp_apply (wp_Everything_weak with "[$Hlabels_init]").
+    iIntros (selector) "%Hselector". wp_auto.
+    wp_apply (wp_State__ReplicaSetList_weak γ model_l
+      rs.(ReplicaSetV.ObjectMeta').(ObjectMetaV.Namespace') selector
+      Hselector with "[$Hapimodel_init $Hisk]").
+    iIntros (replica_sets_sl replica_set_ptrs replica_sets)
+      "(Hreplica_sets_sl & Hreplica_sets & %Hreplica_sets_valid)".
+    wp_auto.
+    iCombineNamed "Hrs_meta_field_*" as "Hrs_meta_fields".
+    iAssert (typed_pointsto_def (ReplicaSetV.objectmeta_ptr rs_l)
+        rs_meta_c dq) with "[Hrs_meta_fields]" as "Hrs_meta_l".
+    { iNamed "Hrs_meta_fields". simpl. rewrite /named.
+      rewrite Hrs_meta_deepown_Hdeepown_namespace. iFrame. }
+    iDestruct (struct_fields_combine (V:=v1.ObjectMeta.t)
+      (ReplicaSetV.objectmeta_ptr rs_l) rs_meta_c dq
+      Hrs_meta_l_nonnull with "Hrs_meta_l") as "Hrs_meta_l".
+    iCombineNamed "Hrs_meta_deepown_*" as "Hrs_meta_deepown".
+    iAssert (ObjectMetaV.deepown rs_meta_c
+        rs.(ReplicaSetV.ObjectMeta') dq)
+      with "[Hrs_meta_deepown]" as "Hrs_meta".
+    { iNamed "Hrs_meta_deepown". rewrite /ObjectMetaV.deepown /named.
+      iFrame. iFrame "%". }
+    iAssert (ObjectMetaV.deepown_l (ReplicaSetV.objectmeta_ptr rs_l)
+        rs.(ReplicaSetV.ObjectMeta') dq) with
+      "[Hrs_meta_l Hrs_meta]" as "Hrs_meta_l".
+    { iExists rs_meta_c. iFrame. }
+    iPoseProof (ReplicaSetV.deepown_l_restore _ _ _ Hrs_l_nonnull with
+      "[$Hrs_typemeta $Hrs_meta_l $Hrs_spec $Hrs_status]") as "Hrs".
+    iDestruct (own_slice_len with "Hreplica_sets_sl") as
+      %(Hreplica_sets_len1 & Hreplica_sets_len2).
+    iDestruct (big_sepL2_length with "Hreplica_sets") as
+      %Hreplica_sets_len.
+    iDestruct (own_slice_wf with "Hreplica_sets_sl") as
+      %Hreplica_sets_cap.
+    wp_apply (wp_slice_make3 (V:=loc)
+      (t:=go.PointerType api_apps_v1.ReplicaSet)); first word.
+    iIntros (related_sl) "(Hrelated_sl & Hrelated_cap & %Hrelated_cap_eq)".
+    wp_auto.
+    set I := (∃ (i : w64) (related_rs_l : loc) (result_sl : slice.t)
+        (result_ptrs : list loc) (result_replica_sets : list ReplicaSetV.t),
+      "Hi_ptr" ∷ i_ptr ↦ i ∗
+      "Hrelated_rs_ptr" ∷ relatedRS_ptr ↦ related_rs_l ∗
+      "Hresult_ptr" ∷ relatedReplicaSets_ptr ↦ result_sl ∗
+      "Hresult_sl" ∷ result_sl ↦* result_ptrs ∗
+      "Hresult_replica_sets" ∷
+        ([∗ list] ptr;replica_set ∈ result_ptrs;result_replica_sets,
+          ReplicaSetV.deepown_l ptr replica_set 1) ∗
+      "Hreplica_sets_post" ∷
+        ([∗ list] ptr;replica_set ∈
+          drop (sint.nat i) replica_set_ptrs;
+          drop (sint.nat i) replica_sets,
+          ReplicaSetV.deepown_l ptr replica_set 1) ∗
+      "Hrelated_cap" ∷ own_slice_cap loc result_sl (DfracOwn 1) ∗
+      "%Hi_bound" ∷
+        ⌜ 0 ≤ sint.Z i ≤ sint.Z (slice.len replica_sets_sl) ⌝)%I.
+    iAssert I with
+      "[i relatedRS relatedReplicaSets Hrelated_sl Hrelated_cap
+        Hreplica_sets]" as "Hloop".
+    { iExists (W64 0), null, related_sl, [], [].
+      iFrame. rewrite !big_sepL2_nil. iFrame.
+      iPureIntro. word. }
+    wp_for "Hloop". wp_if_destruct.
+    + list_elem replica_set_ptrs (sint.Z i) as this_ptr.
+      destruct (decide
+        (0 ≤ sint.Z i < sint.Z (slice.len replica_sets_sl))) as
+        [_|Hbounds]; last word.
+      wp_apply (wp_load_slice_index with "[$Hreplica_sets_sl]");
+        [word|iPureIntro; exact Hthis_ptr_lookup|].
+      iIntros "Hreplica_sets_sl". wp_auto.
+      assert (∃ this_rs, replica_sets !! sint.nat i = Some this_rs) as
+        [this_rs Hthis_rs_lookup].
+      { apply lookup_lt_is_Some_2.
+        rewrite -Hreplica_sets_len Hreplica_sets_len1. word. }
+      iPoseProof (big_sepL2_head_tail _ _ _ this_ptr this_rs with
+        "Hreplica_sets_post") as "[Hthis Hother]".
+      { split. all: rewrite lookup_drop Nat.add_0_r; done. }
+      wp_bind (@! v1.GetControllerOf
+        #(interface.mk_ok (go.PointerType api_apps_v1.ReplicaSet)
+          #this_ptr))%E.
+      wp_apply (wp_GetControllerOf_ReplicaSet with
+        "[$Hmeta_init $Hthis //]").
+      iIntros (related_controller_ref_l)
+        "(Hthis & Hrelated_controller_ref)".
+      iDestruct "Hrelated_controller_ref" as
+        "[%Hrelated_controller_ref_null|Hrelated_controller_ref]".
+      * subst related_controller_ref_l. wp_auto.
+        iApply wp_for_post_do. wp_auto.
+        iFrame "Hreplica_sets_sl HΦ Hrs Hcontroller_var Hcontroller_uid
+          Hcontroller_rest".
+        iExists (word.add i (W64 1)), this_ptr, result_sl,
+          result_ptrs, result_replica_sets.
+        assert (sint.nat (word.add i (W64 1)) = S (sint.nat i)) as
+          -> by word.
+        rewrite !drop_drop Nat.add_1_r. iFrame. iPureIntro. word.
+      * iDestruct "Hrelated_controller_ref" as (related_controller_ref)
+          "(%Hrelated_controller_ref & Hrelated_controller_ref)".
+        destruct Hrelated_controller_ref as
+          [Hrelated_controller_ref_nonnull Hrelated_controller_ref_of].
+        wp_auto.
+        rewrite -> bool_decide_false by
+          exact Hrelated_controller_ref_nonnull.
+        wp_auto.
+        iDestruct "Hrelated_controller_ref" as
+          (related_controller_ref_c)
+          "[Hrelated_controller_ref_l Hrelated_controller_ref]".
+        iDestruct (struct_fields_split (V:=v1.OwnerReference.t) with
+          "Hrelated_controller_ref_l") as
+          "[Hrelated_controller_ref_fields %Hrelated_controller_ref_l_nonnull]".
+        iNamedPrefix "Hrelated_controller_ref_fields"
+          "Hrelated_controller_ref_field_".
+        iNamedPrefix "Hrelated_controller_ref"
+          "Hrelated_controller_ref_deepown_".
+        wp_auto.
+        rewrite Hrelated_controller_ref_deepown_Hdeepown_uid
+          Hcontroller_ref_deepown_Hdeepown_uid.
+        wp_if_destruct.
+        -- wp_apply wp_slice_literal. iSplitR; first done.
+           iIntros (one_sl) "[Hone_sl _]". wp_auto.
+           wp_apply (wp_slice_append with
+             "[$Hresult_sl $Hrelated_cap $Hone_sl]").
+           iIntros (result_sl')
+             "(Hresult_sl & Hrelated_cap & Hone_sl)". wp_auto.
+           iAssert (([∗ list] ptr;replica_set ∈
+               result_ptrs ++ [this_ptr];
+               result_replica_sets ++ [this_rs],
+               ReplicaSetV.deepown_l ptr replica_set 1))%I
+             with "[Hresult_replica_sets Hthis]" as
+             "Hresult_replica_sets".
+           { iApply (big_sepL2_app with "[$Hresult_replica_sets]").
+             simpl. iFrame. }
+           iApply wp_for_post_do. wp_auto.
+           iFrame "Hreplica_sets_sl HΦ Hrs Hcontroller_var Hcontroller_uid
+             Hcontroller_rest".
+           iExists (word.add i (W64 1)), this_ptr, result_sl',
+             (result_ptrs ++ [this_ptr]),
+             (result_replica_sets ++ [this_rs]).
+           assert (sint.nat (word.add i (W64 1)) = S (sint.nat i))
+             as -> by word.
+           rewrite !drop_drop Nat.add_1_r.
+           iFrame. iPureIntro. word.
+        -- iApply wp_for_post_do. wp_auto.
+           iFrame "Hreplica_sets_sl HΦ Hrs Hcontroller_var Hcontroller_uid
+             Hcontroller_rest".
+           iExists (word.add i (W64 1)), this_ptr, result_sl,
+             result_ptrs, result_replica_sets.
+           assert (sint.nat (word.add i (W64 1)) = S (sint.nat i))
+             as -> by word.
+           rewrite !drop_drop Nat.add_1_r. iFrame. iPureIntro. word.
+    + clear I.
+      iApply ("HΦ" $! result_sl result_ptrs result_replica_sets
+        (DfracOwn 1)).
+      iFrame.
+Qed.
+
+End proof.
