src/proof/k8s_io/api/apps/v1.v
@@ -1,5 +1,6 @@
 From New.proof.k8s_io.api.apps Require Export v1_init.
 From New.proof.k8s_io.apimachinery.pkg.runtime Require Export schema.
+From New.proof.k8s_io.apimachinery.pkg.apis.meta Require Export v1.
 
 From New.proof Require Import prelude empty_ffi.
 From New.proof.kubernetes_types Require Import prelude.
@@ -37,6 +38,61 @@ Proof using hG schema_sem sem Σ.
   rewrite Hgroup Hversion HSchemeGroupVersion_Group
     HSchemeGroupVersion_Version.
   done.
+Qed.
+
+Context {meta_v1_sem : code.k8s_io.apimachinery.pkg.apis.meta.v1.v1.Assumptions}
+  {core_v1_sem : code.k8s_io.api.core.v1.v1.Assumptions}
+  {apps_v1_sem : code.k8s_io.api.apps.v1.v1.Assumptions}.
+Local Set Default Proof Using "All".
+
+Lemma get_owner_references_capability_ReplicaSet rs_l rs dq :
+  ⊢ get_owner_references_capability
+    (interface.mk_ok (go.PointerType api_apps_v1.ReplicaSet) #rs_l)
+    rs.(ReplicaSetV.ObjectMeta') dq
+    (ReplicaSetV.deepown_l rs_l rs dq).
+Proof.
+  unfold get_owner_references_capability.
+  wp_start as "H". iNamed "H".
+  iPoseProof (ReplicaSetV.deepown_l_split with "Hown") as
+    "(%Hrs_l_nonnull & Htypemeta & Hmeta & Hspec & Hstatus)".
+  wp_auto.
+  wp_method_call.
+  wp_pures.
+  wp_apply (wp_GetOwnerReferences_deepown with "[$Hinit $Hmeta]").
+  iIntros (sl) "(%Hnil & Hrefs)".
+  iApply "HΦ". iSplit; first done.
+  destruct rs.(ReplicaSetV.ObjectMeta').(ObjectMetaV.OwnerReferences') as
+    [refs|] eqn:Hrefs_some.
+  - iDestruct "Hrefs" as (cs) "(Hsl & Hrefs & Hmeta_restore)".
+    iExists cs. iFrame "Hsl Hrefs".
+    iIntros (cs') "[Hsl Hrefs]".
+    iDestruct ("Hmeta_restore" with "[$Hsl $Hrefs]") as "Hmeta".
+    iApply (ReplicaSetV.deepown_l_restore _ _ _ Hrs_l_nonnull).
+    iFrame.
+  - iApply (ReplicaSetV.deepown_l_restore _ _ _ Hrs_l_nonnull).
+    iFrame.
+Qed.
+
+Lemma wp_GetControllerOf_ReplicaSet owner rs_l rs dq :
+  {{{ "Hinit" ∷ is_pkg_init v1 ∗
+      "%Howner" ∷ ⌜ owner = interface.mk_ok (go.PointerType api_apps_v1.ReplicaSet) #rs_l ⌝ ∗
+      "Hrs" ∷ ReplicaSetV.deepown_l rs_l rs dq
+  }}}
+    @! v1.GetControllerOf #owner
+  {{{ controller_ref_l, RET #controller_ref_l;
+      ReplicaSetV.deepown_l rs_l rs dq ∗
+      (⌜ controller_ref_l = null ⌝ ∨
+       ∃ controller_ref,
+         ⌜ controller_ref_l ≠ null ∧
+           is_controller_reference_of rs.(ReplicaSetV.ObjectMeta') controller_ref ⌝ ∗
+         OwnerReferenceV.deepown_l controller_ref_l controller_ref 1)
+  }}}.
+Proof.
+  iIntros (Φ) "H HΦ". iNamed "H". subst owner.
+  iPoseProof (get_owner_references_capability_ReplicaSet rs_l rs dq) as
+    "Hget".
+  iApply (wp_GetControllerOf_general with "[$Hinit $Hget $Hrs]").
+  iExact "HΦ".
 Qed.
 
 End proof.
